# Complete Guide to Mathematical Proof Methods

## 1.7.1 Introduction to Proofs

### What is a Proof?
A **proof** is a valid argument that establishes the truth of a mathematical statement. A proof uses:
- **Hypotheses** of the theorem (if any)
- **Axioms** assumed to be true
- **Previously proven theorems**
- **Rules of inference** to connect logical steps

### Types of Proofs

#### Formal Proofs
- All steps are explicitly supplied
- Rules for each step are clearly stated
- Used by computers and automated reasoning systems
- Often extremely long and difficult for humans to follow

#### Informal Proofs
- Multiple rules of inference may be used in each step
- Some steps may be skipped
- Axioms and rules are not always explicitly stated
- Designed for human understanding
- More common in practice

### Applications
Proof methods are essential in:
- Mathematics
- Computer science (program verification)
- Operating system security
- Artificial intelligence
- System specification consistency

## 1.7.2 Mathematical Terminology

### Key Definitions

#### Theorem
- A statement that can be shown to be true
- Usually reserved for somewhat important results
- May be a universal quantification: ∀x(P(x) → Q(x))

#### Proposition
- A less important theorem
- Sometimes called facts or results

#### Lemma (plural: lemmas or lemmata)
- A less important theorem that helps prove other results
- Building blocks for complex proofs
- Each lemma is proved individually

#### Corollary
- A theorem that follows directly from a previously proven theorem
- Usually an immediate consequence

#### Conjecture
- A proposed statement believed to be true
- Based on partial evidence, heuristic arguments, or intuition
- Becomes a theorem when proved
- May be shown false (then it's not a theorem)

#### Axiom (or Postulate)
- Statements assumed to be true
- Examples: axioms for real numbers, plane geometry
- May use primitive terms that don't require definition
- All other terms must be defined

## 1.7.3 Understanding Theorem Statements

### Universal Quantifiers in Theorems

Many theorems assert properties for all elements in a domain, but the universal quantifier is often omitted by convention.

**Example:**
- **Stated:** "If x > y, where x and y are positive real numbers, then x² > y²"
- **Actually means:** "For all positive real numbers x and y, if x > y, then x² > y²"

### Proof Structure for Universal Statements
1. Select a general element of the domain
2. Show this element has the required property
3. Universal generalization implies the theorem holds for all domain members

## 1.7.4 Methods of Proving Theorems

### General Strategy
To prove ∀x(P(x) → Q(x)):
1. Show P(c) → Q(c) for arbitrary element c
2. Apply universal generalization

### Focus on Conditional Statements
Since p → q is false only when p is true and q is false, we need to show:
- If p is true, then q must also be true

## 1.7.5 Direct Proofs

### Definition
A **direct proof** of p → q:
1. Assume p is true
2. Use axioms, definitions, and proven theorems
3. Apply rules of inference
4. Show q must be true

### Key Definitions for Examples

**Definition 1:** 
- Integer n is **even** if ∃ integer k such that n = 2k
- Integer n is **odd** if ∃ integer k such that n = 2k + 1
- Every integer is either even or odd, never both
- **Same parity:** both even or both odd
- **Opposite parity:** one even, one odd

### Example 1: Odd Integer Squared
**Theorem:** If n is an odd integer, then n² is odd.

**Direct Proof:**
1. **Assume:** n is odd
2. **By definition:** n = 2k + 1 for some integer k
3. **Square both sides:** n² = (2k + 1)²
4. **Expand:** n² = 4k² + 4k + 1 = 2(2k² + 2k) + 1
5. **Conclude:** n² is odd (form 2m + 1 where m = 2k² + 2k)

### Example 2: Product of Perfect Squares
**Theorem:** If m and n are both perfect squares, then mn is also a perfect square.

**Definition:** Integer a is a perfect square if ∃ integer b such that a = b².

**Direct Proof:**
1. **Assume:** m and n are perfect squares
2. **By definition:** m = s² and n = t² for integers s, t
3. **Multiply:** mn = s²t² = (st)²
4. **Conclude:** mn is a perfect square (st is an integer)

## 1.7.6 Proof by Contraposition

### Definition
**Proof by contraposition** uses the logical equivalence:
p → q ≡ ¬q → ¬p

### Method
To prove p → q:
1. Assume ¬q (negation of conclusion)
2. Use axioms, definitions, and theorems
3. Show ¬p must follow

### Example 3: Contraposition with Odd Numbers
**Theorem:** If n is an integer and 3n + 2 is odd, then n is odd.

**Attempted Direct Proof:**
- Assume 3n + 2 is odd, so 3n + 2 = 2k + 1
- Then 3n + 1 = 2k
- No clear way to show n is odd

**Proof by Contraposition:**
1. **Assume:** n is even (¬"n is odd")
2. **By definition:** n = 2k for some integer k
3. **Substitute:** 3n + 2 = 3(2k) + 2 = 6k + 2 = 2(3k + 1)
4. **Conclude:** 3n + 2 is even, so not odd
5. **Result:** ¬(conclusion) → ¬(hypothesis), proving the original statement

### Example 4: Square Root Inequality
**Theorem:** If n = ab where a and b are positive integers, then a ≤ √n or b ≤ √n.

**Proof by Contraposition:**
1. **Assume:** ¬(a ≤ √n or b ≤ √n)
2. **By De Morgan's law:** a > √n and b > √n
3. **Multiply inequalities:** ab > √n · √n = n
4. **Contradiction:** ab ≠ n, but we assumed n = ab
5. **Conclude:** Original statement is true

## 1.7.7 Vacuous and Trivial Proofs

### Vacuous Proof
**When:** The hypothesis p is false
**Result:** p → q is automatically true
**Use:** Often for special cases of theorems

### Example 5: Vacuous Proof
**Show:** P(0) is true, where P(n) is "If n > 1, then n² > n" (domain: all integers)

**Solution:**
- P(0): "If 0 > 1, then 0² > 0"
- Hypothesis "0 > 1" is false
- Therefore P(0) is automatically true (vacuous proof)

### Example 6: Perfect Squares
**Theorem:** If n is an integer with 10 ≤ n ≤ 15 which is a perfect square, then n is also a perfect cube.

**Solution:**
- No perfect squares exist with 10 ≤ n ≤ 15 (since 3² = 9 and 4² = 16)
- Hypothesis is false for all integers n
- Statement is vacuously true

### Trivial Proof
**When:** The conclusion q is true
**Result:** p → q is automatically true

### Example 7: Trivial Proof
**Show:** P(0) is true, where P(n) is "If a ≥ b, then aⁿ ≥ bⁿ" for positive integers a, b

**Solution:**
- P(0): "If a ≥ b, then a⁰ ≥ b⁰"
- Since a⁰ = b⁰ = 1, conclusion "a⁰ ≥ b⁰" is true
- Therefore P(0) is true (trivial proof)

## 1.7.8 Proof Strategy Guidelines

### When to Use Direct Proof
1. Expand definitions in hypotheses
2. Start reasoning from hypotheses
3. If clear path to conclusion exists, continue with direct proof

### When to Try Contraposition
1. Direct proof doesn't seem to work
2. No clear way to use hypotheses
3. Hypotheses like "x is irrational" or "x ≠ 0" are difficult to reason from
4. Often easier when negation of conclusion is more manageable

### Definition for Rational Numbers

**Definition 2:** 
- Real number r is **rational** if ∃ integers p, q with q ≠ 0 such that r = p/q
- A real number that is not rational is **irrational**

### Example 8: Sum of Rational Numbers
**Theorem:** The sum of two rational numbers is rational.

**Direct Proof:**
1. **Assume:** r and s are rational
2. **By definition:** r = p/q and s = t/u where p,q,t,u are integers, q ≠ 0, u ≠ 0
3. **Add:** r + s = p/q + t/u = (pu + qt)/(qu)
4. **Check:** pu + qt and qu are integers, qu ≠ 0
5. **Conclude:** r + s is rational

### Example 9: Even Square Implies Even
**Theorem:** If n is an integer and n² is odd, then n is odd.

**Direct Proof Attempt:**
- Assume n² is odd, so n² = 2k + 1
- Solving gives n = ±√(2k + 1), which isn't useful

**Proof by Contraposition:**
1. **Assume:** n is not odd, so n is even
2. **By definition:** n = 2k for some integer k
3. **Square:** n² = 4k² = 2(2k²)
4. **Conclude:** n² is even (not odd)

## 1.7.9 Proofs by Contradiction

### Method
To prove statement p:
1. Assume ¬p is true
2. Show this leads to a contradiction q ∧ ¬q
3. Since contradiction is impossible, ¬p must be false
4. Therefore p is true

### Example 10: Pigeonhole Principle Application
**Theorem:** At least four of any 22 days must fall on the same day of the week.

**Proof by Contradiction:**
1. **Assume:** At most three of the 22 days fall on the same day of week
2. **Analysis:** 7 days of week × at most 3 days each = at most 21 days
3. **Contradiction:** We have 22 days, but can account for at most 21
4. **Conclude:** Original statement is true

### Example 11: √2 is Irrational
**Theorem:** √2 is irrational.

**Proof by Contradiction:**
1. **Assume:** √2 is rational
2. **Then:** √2 = a/b where a,b are integers with no common factors, b ≠ 0
3. **Square:** 2 = a²/b², so 2b² = a²
4. **Analysis:** a² is even, so a is even
5. **Let:** a = 2c for integer c
6. **Substitute:** 2b² = 4c², so b² = 2c²
7. **Analysis:** b² is even, so b is even
8. **Contradiction:** Both a and b are even (have common factor 2), but we assumed they had no common factors
9. **Conclude:** √2 is irrational

### Example 12: Rewriting Contraposition as Contradiction
**Theorem:** If 3n + 2 is odd, then n is odd.

**Proof by Contradiction:**
1. **Assume:** 3n + 2 is odd AND n is not odd
2. **Since n is not odd:** n is even, so n = 2k
3. **Substitute:** 3n + 2 = 6k + 2 = 2(3k + 1)
4. **Result:** 3n + 2 is even
5. **Contradiction:** 3n + 2 is both odd (assumption) and even
6. **Conclude:** Original statement is true

## 1.7.10 Proofs of Equivalence

### Biconditional Statements
To prove p ↔ q, show both:
- p → q
- q → p

### Example 13: Odd Integer Equivalence
**Theorem:** If n is an integer, then n is odd if and only if n² is odd.

**Proof:**
1. **Part 1 (n odd → n² odd):** Already proved in Example 1
2. **Part 2 (n² odd → n odd):** Already proved in Example 9
3. **Conclude:** Both directions proven, so equivalence holds

### Multiple Equivalences
To prove p₁ ↔ p₂ ↔ ... ↔ pₙ, show chain:
p₁ → p₂, p₂ → p₃, ..., pₙ → p₁

### Example 14: Three Equivalent Statements
**Theorem:** These statements about integer n are equivalent:
- p₁: n is even
- p₂: n - 1 is odd  
- p₃: n² is even

**Proof Chain: p₁ → p₂ → p₃ → p₁**

**Prove p₁ → p₂:**
1. Assume n is even, so n = 2k
2. Then n - 1 = 2k - 1 = 2(k-1) + 1
3. So n - 1 is odd

**Prove p₂ → p₃:**
1. Assume n - 1 is odd, so n - 1 = 2k + 1
2. Then n = 2k + 2
3. So n² = (2k + 2)² = 4k² + 8k + 4 = 2(2k² + 4k + 2)
4. Therefore n² is even

**Prove p₃ → p₁ (by contraposition):**
1. If n is odd, then n² is odd (proved in Example 1)
2. Contrapositive: if n² is even, then n is even

## 1.7.11 Counterexamples

### Purpose
To show ∀xP(x) is false, find one example where P(x) is false.

### Example 15: Counterexample
**Statement:** "Every positive integer is the sum of the squares of two integers."

**Counterexample:**
- Consider n = 3
- Perfect squares ≤ 3: 0² = 0, 1² = 1
- Possible sums: 0+0=0, 0+1=1, 1+1=2
- Cannot get 3 as sum of two perfect squares
- Therefore statement is false

## 1.7.12 Common Mistakes in Proofs

### Example 16: Division by Zero Error
**False "Proof" that 1 = 2:**
1. a = b (given)
2. a² = ab (multiply by a)
3. a² - b² = ab - b² (subtract b²)
4. (a-b)(a+b) = b(a-b) (factor)
5. a + b = b (divide by a-b) ← **ERROR!**
6. 2b = b (since a = b)
7. 2 = 1 (divide by b)

**Error:** Step 5 divides by (a-b) = 0, which is invalid.

### Example 17: Affirming the Conclusion
**False "Theorem":** If n² is positive, then n is positive.
**False "Proof":** Since "n positive → n² positive" is true, and n² is positive, we conclude n is positive.

**Error:** This is the fallacy of affirming the conclusion. Counterexample: n = -1 gives n² = 1 > 0, but n < 0.

### Example 18: Denying the Hypothesis  
**False "Theorem":** If n is not positive, then n² is not positive.
**False "Proof":** Since "n positive → n² positive" is true, and n is not positive, we conclude n² is not positive.

**Error:** This is the fallacy of denying the hypothesis. Same counterexample: n = -1.

### Example 19: Circular Reasoning
**False "Proof":** If n² is even, then n is even.
**Attempt:** Suppose n² is even, so n² = 2k. Let n = 2l for some integer l. Therefore n is even.

**Error:** The statement "let n = 2l" assumes what we're trying to prove (that n is even). This is circular reasoning or "begging the question."

## Key Takeaways

### Proof Method Selection
1. **Try direct proof first** if hypotheses clearly lead toward conclusion
2. **Use contraposition** when:
   - Direct proof gets stuck
   - Negation of conclusion is easier to work with
   - Hypotheses involve negatives or irrationals
3. **Use contradiction** when:
   - Both direct and contraposition fail
   - Statement seems obviously true but hard to prove directly

### Common Proof Structure
1. **State what you're proving**
2. **Choose appropriate method**
3. **Set up assumptions clearly**
4. **Use definitions, axioms, and previous results**
5. **Show each step follows logically**
6. **State conclusion clearly**

### Avoiding Errors
- **Check arithmetic carefully**
- **Ensure each step follows logically**
- **Don't divide by expressions that could be zero**
- **Avoid logical fallacies**
- **Don't use circular reasoning**
- **Provide counterexamples for false statements**

This foundation provides the essential tools for mathematical reasoning and proof construction across all areas of mathematics and computer science.
